feat: start implementing Framework for Domain n Sign

lean-formalisation/LeanFormalisation/LBase/LBaseCFG/Positivity.lean
@@ -2,7 +2,10 @@ import LeanFormalisation.LBase.LBaseCFG.AltCFG
 import LeanFormalisation.LBase.LBaseCFG.Analysis
 import LeanFormalisation.LBase.LBaseCFG.AltCFGRepr
 
-open LeanFormalisation AltCFG
+import LeanFormalisation.LBase.LBaseCFG.Framework
+import LeanFormalisation.LBase.LBaseCFG.CorrespondenceProofs
+
+open LeanFormalisation AltCFG AltCFGProofs
 
 section Sign
 inductive Sign where
@@ -28,6 +31,7 @@ instance : Repr Sign where
     | .Bot => "∅"
     | .Top => "ℕ"
 
+@[simp]
 private def Sign.fromAtomFlags (hasNeg hasZero hasPos : Bool) : Sign :=
   match hasNeg, hasZero, hasPos with
   | false, false, false => .Bot
@@ -73,9 +77,18 @@ def Sign.inf : Sign → Sign → Sign
 instance : Max Sign where
   max := Sign.sup
 
+lemma Sign.sup_comm {a b : Sign} : a ⊔ b = b ⊔ a := by
+  simp only [max, Sign.sup, Sign.hasNeg, Sign.hasZero, Sign.hasPos]
+  cases a <;> simp
+
+lemma Sign.sup_assoc {a b c : Sign} : a ⊔ (b ⊔ c) = (a ⊔ b) ⊔ c := by
+  simp only [max, Sign.sup, Sign.hasNeg, Sign.hasZero, Sign.hasPos]
+  cases a <;> cases b <;> cases c <;> simp
+
 instance : Min Sign where
   min := Sign.inf
 
+@[simp]
 def Sign.addAtomic : Sign → Sign → Sign
 | .Pos, .Pos => .Pos
 | .Pos, .Zero => .Pos
@@ -88,6 +101,7 @@ def Sign.addAtomic : Sign → Sign → Sign
 | .Neg, .Neg => .Neg
 | _, _ => .Top
 
+@[simp]
 def Sign.subAtomic : Sign → Sign → Sign
 | .Pos, .Pos => .Top
 | .Pos, .Zero => .Pos
@@ -100,6 +114,7 @@ def Sign.subAtomic : Sign → Sign → Sign
 | .Neg, .Neg => .Top
 | _, _ => .Top
 
+@[simp]
 private def Sign.atomicChoices : Sign → List Sign
 | .Pos => [.Pos]
 | .Neg => [.Neg]
@@ -109,19 +124,26 @@ private def Sign.atomicChoices : Sign → List Sign
 | .Top => [.Neg, .Zero, .Pos]
 | .Bot => []
 
+@[simp]
 private def Sign.foldSup (xs : List Sign) : Sign :=
   xs.foldl (fun acc s => acc ⊔ s) .Bot
 
+@[simp]
 private def Sign.combineAtomic (op : Sign → Sign → Sign)
     (lhs rhs : List Sign) : Sign :=
   lhs.foldl
     (fun acc a => rhs.foldl (fun acc' b => acc' ⊔ op a b) acc)
     .Bot
 
+@[simp]
 def Sign.add : Sign → Sign → Sign
 | s₁, s₂ =>
   Sign.combineAtomic Sign.addAtomic s₁.atomicChoices s₂.atomicChoices
 
+lemma Sign.add_comm (a b : Sign) : a.add b = b.add a := by
+  cases a <;> cases b <;> simp [Sign.add, max, Sign.sup]
+
+@[simp]
 def Sign.sub : Sign → Sign → Sign
 | s₁, s₂ =>
   Sign.combineAtomic Sign.subAtomic s₁.atomicChoices s₂.atomicChoices
@@ -172,6 +194,144 @@ def evalExprSign {n : Nat} (ρ : Domain n Sign) : Lang .Expr -> Sign
 | .While _ _
 | .Break _ => .Top
 
+set_option maxHeartbeats 240000 in
+-- it seems that the default 200000 is just barely not enough to find this proof
+-- and i cannot be arsed to optimize for a better one.
+lemma Sign.add_mono_right (a b c : Sign) (h : a ⊔ b = a) :
+    a.add c ⊔ b.add c = a.add c := by
+  -- cases a <;> cases b <;> cases c <;> simp [max, Sign.sup] at h ⊢
+  sorry
+
+lemma Sign.add_mono (a b c d : Sign) (h₁ : a ⊔ b = a) (h₂ : c ⊔ d = c) :
+    a.add c ⊔ b.add d = a.add c := by
+  have int₁ := add_mono_right _ _ c h₁
+  have int₂ := add_mono_right _ _ a h₂
+  calc
+  a.add c ⊔ b.add d
+      = (a.add c ⊔ b.add c) ⊔ b.add d := by
+          conv => lhs; rw [<- int₁]
+  _   = a.add c ⊔ (b.add c ⊔ b.add d) := by
+          rw [Sign.sup_assoc]
+  _   = a.add c ⊔ b.add c := by
+          rw [Sign.add_comm b c, Sign.add_comm b d, add_mono_right c d b h₂]
+  _   = a.add c := int₁
+
+set_option maxHeartbeats 240000 in
+-- et simile
+lemma Sign.sub_mono_right (a b c : Sign) (h : a ⊔ b = a) :
+    a.sub c ⊔ b.sub c = a.sub c := by
+  -- cases a <;> cases b <;> cases c <;> simp [max, Sign.sup] at h ⊢
+  sorry
+
+set_option maxHeartbeats 400000 in
+-- et simile
+lemma Sign.sub_mono_left (a b c : Sign) (h : c ⊔ b = c) :
+    a.sub c ⊔ a.sub b = a.sub c := by
+  -- cases a <;> cases b <;> cases c <;> simp [max, Sign.sup] at h ⊢
+  sorry
+
+set_option maxHeartbeats 1000000 in
+-- needs big simp
+-- provable but slow. isok.
+lemma Sign.sub_mono (a b c d : Sign) (h₁ : a ⊔ b = a) (h₂ : c ⊔ d = c) :
+    a.sub c ⊔ b.sub d = a.sub c := by
+  have int₁ := Sign.sub_mono_right a b d h₁
+  have int₂ := Sign.sub_mono_left a d c h₂
+  calc
+    a.sub c ⊔ b.sub d = (a.sub c ⊔ a.sub d) ⊔ b.sub d := by
+      exact congrArg (fun x => x ⊔ b.sub d) (Eq.symm int₂)
+    _ = a.sub c ⊔ (a.sub d ⊔ b.sub d) := by
+      symm
+      rw [Sign.sup_assoc]
+    _ = a.sub c ⊔ a.sub d := by
+      rw [int₁]
+    _ = a.sub c := int₂
+
+lemma Sign.meet_mono {a b c : Sign} (h : a ⊔ b = a) :
+    (a ⊓ c) ⊔ (b ⊓ c) = a ⊓ c := by
+  cases a <;> cases b <;> cases c <;>
+    simp [max, Sign.sup, min, Sign.inf] at h ⊢
+
+lemma Sign.meet_bot_right {x : Sign} :
+    x ⊓ ⊥ = ⊥ := by
+  cases x <;> simp [min, Sign.inf] <;> rfl
+
+lemma Sign.meet_eq_of_join_right {a b c : Sign} (h : a ⊔ b = b) (hc : c ⊓ a = c) :
+    c ⊓ b = c := by
+  cases a <;> cases b <;> cases c <;>
+    simp [max, Sign.sup, min, Sign.inf] at h hc ⊢
+
+-- fake motive to apply false indcution.
+def M (n : Nat) : (t : Tag) → Lang t → Prop
+| .Expr, e =>
+    ∀ x y : Domain n Sign, x ⊔ y = x →
+      evalExprSign x e ⊔ evalExprSign y e = evalExprSign x e
+| .Stmt, _ => True
+
+lemma evalExprSign_mono {n : Nat} : ∀ e : Lang .Expr, M n .Expr e := by
+  intro e
+  refine (Lang.rec (motive := M n)
+    ?hVar ?hTrue ?hFalse ?hNat ?hUnit ?hBinOp ?hUnOp ?hIf ?hWhile ?hBreak ?hScope
+    ?hDecl ?hAssign ?hSeq ?hDo) e
+  · intro x ρ₁ ρ₂ hxy
+    simp [evalExprSign, getVar]
+    by_cases h : x < n
+    · simpa [h, max, Sign.fromAtomFlags] using congrFun hxy ⟨x, by assumption⟩
+    · simp only [h, ↓reduceDIte]; rfl
+  · intro x y hxy
+    simp [evalExprSign, max, Sign.fromAtomFlags]
+  · intro x y hxy
+    simp [evalExprSign, max, Sign.fromAtomFlags]
+  · intro n x y hxy
+    simp only [max, Sign.sup, Sign.fromAtomFlags, Sign.hasNeg, evalExprSign, signOfNat,
+      Bool.or_self, Sign.hasZero, Sign.hasPos]
+    cases n <;> simp
+  · intro x y hxy
+    simp [evalExprSign, max, Sign.fromAtomFlags]
+  · intro e₁ e₂ op ih₁ ih₂ ρ₁ ρ₂ hxy
+    specialize ih₁ _ _ hxy
+    specialize ih₂ _ _ hxy
+    cases op <;> simp only [evalExprSign]
+    · grind [Sign.add_mono]
+    · grind [Sign.sub_mono]
+    · simp [max]
+    · simp [max]
+  · intros a o ih
+    intros x y hxy
+    specialize ih x y hxy
+    cases o <;> simp [evalExprSign, max, Sign.fromAtomFlags]
+  · intros c e₁ e₂ _ ih₁ ih₂
+    intros x y hxy
+    specialize ih₁ x y hxy
+    specialize ih₂ x y hxy
+    unfold evalExprSign
+    calc
+      evalExprSign x e₁ ⊔ evalExprSign x e₂ ⊔
+        (evalExprSign y e₁ ⊔ evalExprSign y e₂)
+        =
+        (evalExprSign x e₁ ⊔ evalExprSign y e₁) ⊔
+        (evalExprSign x e₂ ⊔ evalExprSign y e₂) := by
+          grind [Sign.sup_comm, Sign.sup_assoc]
+      _ = evalExprSign x e₁ ⊔ evalExprSign x e₂ := by
+        simp [ih₁, ih₂]
+  · intros c b ihc ihb
+    intros x y hxy
+    simp [evalExprSign, max, Sign.fromAtomFlags]
+  · intros l x y hxy
+    simp [evalExprSign, max, Sign.fromAtomFlags]
+  · intros s res ihs ihres
+    intros x y hxy
+    unfold evalExprSign
+    exact ihres _ _ hxy
+  · intros; simp only [M]
+  · intros; simp only [M]
+  · intros; simp only [M]
+  · intros; simp only [M]
+
+lemma excludeZero_mono {a b : Sign} (h : a ⊔ b = a) :
+    a.excludeZero ⊔ b.excludeZero = a.excludeZero := by
+  cases a <;> cases b <;> simp [Sign.excludeZero, max] at h ⊢
+
 def transferPosNode {n : Nat} (node : CFGNode) (ρ : Domain n Sign) : Domain n Sign :=
   transferScopedNode evalExprSign node ρ
 
@@ -196,6 +356,238 @@ def transferPosEdge {n : Nat} (e : CFGEdge) (ρ : Domain n Sign) : Domain n Sign
 def runPositivity (n : Nat) (g : CFG)
     (entryInit : Domain n Sign := ⊥) : PosFact n g × PosFact n g :=
   runDataflowOf g transferPosNode transferPosEdge entryInit
+
+instance {s} : TranslationReq s (cfgcekRel s) := (cfgcekRelReq s (by sorry))
+
+def absPos : CEK -> Domain n Sign -> Prop := fun σ ρ =>
+  σ.E.length ≤ n ∧
+  ∀ x : Fin n,
+    let concreteSign : Sign :=
+      if h : x.val < σ.E.length then
+        match σ.E[x.val] with
+        | .Nat 0 => Sign.Zero
+        | .Nat _ => Sign.Pos
+        | .True | .False | .Unit => Sign.Top
+      else
+        Sign.Bot -- unreachable?
+    concreteSign ⊓ (getVar ρ x.val) = concreteSign
+
+theorem absPos_mono {σ : CEK} {a b : Domain n Sign}
+    (hab : a ⊔ b = b) (habsa : absPos σ a) :
+    absPos σ b := by
+  obtain ⟨hlen, habsa⟩ := habsa
+  refine ⟨hlen, ?_⟩
+  intro x
+  simp only [getVar, Fin.is_lt, ↓reduceDIte, Fin.eta]
+  refine Sign.meet_eq_of_join_right (congrFun hab x) ?_
+  simpa [getVar] using (habsa x)
+
+lemma positivity_step_sound_core {s σ σ' nod nod'}
+    (hrel : cfgcekRel s σ nod)
+    (hrel' : cfgcekRel s σ' nod')
+    (heval : Eval σ σ')
+    (hreach : CFGReach (stmtCFG s) nod nod')
+    (hfact : GFact (stmtCFG s) (Domain n Sign))
+    (habs : absPos σ (hfact nod)) :
+    absPos σ' (transferPosNode nod'.val
+      (expectedInOf (stmtCFG s) transferPosEdge (fun _ => ⊥) hfact nod')) := by
+  sorry
+
+instance : Framework (Domain n Sign) transferPosEdge transferPosNode s (cfgcekRel s) absPos where
+  join_comm := fun a b => by
+    funext x
+    simp only [max, Sign.sup, Sign.hasNeg, Sign.hasZero, Sign.hasPos]
+    cases (a x) <;> simp
+  join_assoc :=  fun a b c => by
+    funext x
+    simp only [max, Sign.sup, Sign.hasNeg, Sign.hasZero, Sign.hasPos, Sign.fromAtomFlags]
+    cases (a x) <;> cases (b x) <;> cases (c x) <;> simp
+  join_idem := fun a => by
+    funext x
+    simp [max, Sign.sup, Sign.fromAtomFlags]
+    cases (a x) <;> simp
+  bot_le := fun a => by
+    funext x
+    simp [max, Sign.sup, Sign.fromAtomFlags]
+    cases (a x) <;> simp
+  node_mono := fun node => by
+    intro x y hxy
+    unfold transferPosNode transferScopedNode
+    cases node.kind with
+    | stmtExit s =>
+      cases s with
+        | Assign x₀ rhs =>
+          funext i
+          simp only [max, setVar]
+          split
+          case isTrue h =>
+            apply evalExprSign_mono
+            exact hxy
+          case isFalse h =>
+            simpa [h, ↓reduceIte] using congrFun hxy _
+        | Decl _ _ =>
+          funext i
+          simp only [max, pushBinding]
+          split
+          case isTrue h =>
+            apply evalExprSign_mono
+            exact hxy
+          case isFalse h =>
+            split
+            case isTrue h' =>
+              apply congrFun hxy
+            case isFalse h' => rfl
+        | _ =>
+          simpa using hxy
+    | exprExit e =>
+      cases e with
+      | Scope s _ =>
+        funext i
+        simp only [max, popBindings]
+        split
+        case isTrue h =>
+          apply congrFun hxy
+        case isFalse h => rfl
+      | _ => simpa using hxy
+    | _ =>
+      simpa using hxy
+  edge_mono := by
+    intro e x y hxy
+    unfold transferPosEdge transferBranchEdge
+    cases e.kind <;> try simpa using hxy
+    · cases e.src.kind <;> try simpa using hxy
+      case exprExit e =>
+      cases e <;> try simpa [refineCond] using hxy
+      case False =>
+        simp only [refineCond]
+        rfl
+      case BinOp a₁ a₂ o =>
+        simp only [refineCond]
+        cases o <;> try simpa using hxy
+        cases a₁ <;> cases a₂ <;> try simpa using hxy
+        case Nat v n =>
+          cases n <;> simp only
+          case zero =>
+            funext i
+            rw [max_app]
+            simp only [setVar]
+            split
+            case isTrue h =>
+              apply Sign.meet_mono
+              have : v < n := by grind
+              simp only [max, Sign.sup, Sign.fromAtomFlags, Sign.hasNeg, getVar, this, ↓reduceDIte,
+                Sign.hasZero, Sign.hasPos]
+              exact congrFun hxy ⟨v, this⟩
+            case isFalse h =>
+              apply congrFun hxy
+          case succ => exact hxy
+        case Var n v =>
+          cases n <;> simp only
+          case zero =>
+            funext i
+            rw [max_app]
+            simp only [setVar]
+            split
+            case isTrue h =>
+              apply Sign.meet_mono
+              have : v < n := by grind
+              simp only [max, Sign.sup, Sign.fromAtomFlags, Sign.hasNeg, getVar, this, ↓reduceDIte,
+                Sign.hasZero, Sign.hasPos]
+              exact congrFun hxy ⟨v, this⟩
+            case isFalse =>
+              apply congrFun hxy
+          case succ => exact hxy
+      case UnOp a o =>
+        simp only [refineCond]
+        cases o <;> cases a <;> try simpa using hxy
+        case Var v =>
+        funext i
+        simp only
+        rw [max_app]
+        simp only [setVar]
+        split
+        case isTrue h =>
+          apply Sign.meet_mono
+          have : v < n := by grind
+          simp only [max, Sign.sup, Sign.fromAtomFlags, Sign.hasNeg, getVar, this, ↓reduceDIte,
+            Sign.hasZero, Sign.hasPos]
+          exact congrFun hxy ⟨v, this⟩
+        case isFalse h =>
+          apply congrFun hxy
+    · cases e.src.kind <;> try simpa using hxy
+      case exprExit e =>
+      cases e <;> try simpa using hxy
+      case True =>
+        simp [refineCond]; rfl
+      case BinOp a₁ a₂ o =>
+        simp only [refineCond]
+        cases o <;> try simpa using hxy
+        cases a₁ <;> cases a₂ <;> try simpa using hxy
+        case Nat v n =>
+          cases n <;> simp only
+          case zero =>
+            funext i
+            rw [max_app]
+            by_cases hi : i.val = v
+            · rw [<- hi]
+              simp only [setVar, ↓reduceIte, getVar]
+              apply excludeZero_mono
+              have : i < n := by grind
+              simpa [this, Max.max] using congrFun hxy i
+            · simp only [max, Sign.sup, Sign.fromAtomFlags, Sign.hasNeg, setVar, hi, ↓reduceIte,
+              Sign.hasZero, Sign.hasPos]
+              exact congrFun hxy i
+          case succ => exact hxy
+        case Var n v =>
+          cases n <;> simp only
+          case zero =>
+            funext i
+            rw [max_app]
+            simp only [setVar]
+            split
+            case isTrue h =>
+              subst h
+              apply excludeZero_mono
+              simp only [getVar]
+              have : i < n := by grind
+              simpa [this, Max.max] using congrFun hxy i
+            case isFalse => apply congrFun hxy
+          case succ => exact hxy
+      case UnOp a o =>
+        simp only [refineCond]
+        cases o <;> cases a <;> try simpa using hxy
+        case Var v =>
+          simp only
+          funext i
+          rw [max_app]
+          simp only [setVar]
+          split
+          case isTrue h =>
+            subst h
+            apply excludeZero_mono
+            simp only [getVar]
+            have : i < n := by grind
+            simpa [this, Max.max] using congrFun hxy i
+          case isFalse h => apply congrFun hxy
+  entryInit := (fun _ => ⊥)
+
+  init_sound := by
+    refine ⟨?_, ?_⟩
+    · simp only [initState, List.length_nil, Nat.zero_le]
+    · simp only [initState, List.length_nil, Nat.not_lt_zero, ↓reduceDIte, getVar, Fin.is_lt]
+      simp [min, Sign.inf]
+  abs_mono := absPos_mono
+
+  abs_preserves_init := by
+    intros a habsa
+    simp only [absPos, initState, List.length_nil, Nat.zero_le, Nat.not_lt_zero, ↓reduceDIte,
+      getVar, Fin.is_lt, Fin.eta, true_and] at habsa ⊢
+    simp [min]
+
+  step_sound := by
+    intros σ σ' nod nod' hrel hrel' heval hreach hfact hfp habs
+    apply absPos_mono (hfp nod')
+    apply positivity_step_sound_core hrel <;> try assumption
 
 def positivityOverlay {n : Nat} {g : CFG} (inF outF : PosFact n g) : AltCFGRepr.DotOverlay :=
   { nodeMeta := fun node =>
